progress

QuantumComputer3Qubits/Formalization/Language.lean
@@ -18,46 +18,156 @@ inductive Cond where
 | c2{i1 i2: Fin 3}{ord: i1 < i2}:  (OP.oi2 i1 i2 ord) → Cond
 | c3:                              OP.o3 → Cond
 
+noncomputable
+def CondSt1{i:Fin 3}(s: StateReg1Ind i): Cond :=
+Cond.c1 (OP s s)
+
+noncomputable
+def CondSt2{i1 i2: Fin 3}{ord: i1 < i2}
+           (s: StateReg2Ind i1 i2 ord): Cond :=
+Cond.c2 (OP s s)
+
+noncomputable
+def CondSt3(s: StateReg3): Cond := Cond.c3 (OP s s)
+
 inductive Prog where
-| skip:                              Prog
-| ass1{i:Fin 3}:                     StateReg1Ind i → Prog
-| ass2{i1 i2: Fin 3}{ord: i1 < i2}:  StateReg2Ind i1 i2 ord → Prog
-| ass3:                              StateReg3 → Prog
-| gate1{i:Fin 3}:                    OP.oi1 i → Prog
-| gate2{i1 i2: Fin 3}{o: i1 < i2}:   OP.oi2 i1 i2 o → Prog
-| gate3:                             OP.o3 → Prog
-| seq:                               Prog → Prog → Prog
+| skip:
+    Prog
+| ass1{i:Fin 3}(s: StateReg1Ind i):
+    Prog
+| ass2{i1 i2: Fin 3}{ord: i1 < i2}(s: StateReg2Ind i1 i2 ord):
+    Prog
+| ass3(s: StateReg3):
+    Prog
+| gate1{i:Fin 3}(op: OP.oi1 i)(un: HC.isUnitary op):
+    Prog
+| gate2{i1 i2: Fin 3}{o: i1 < i2}
+       (op: OP.oi2 i1 i2 o)(un: HC.isUnitary op):
+    Prog
+| gate3(op: OP.o3)(un: HC.isUnitary op):
+    Prog
+| seq(p1 p2: Prog):
+    Prog
 
 inductive Inf: Cond → Prog → Cond → Prop
+
 | Ax.Sk:   ∀h: Cond, Inf h Prog.skip h
-| Ax.UTF1(i: Fin 3):
-    ∀op tr: (OP.oi1 i),
+
+| Ax.UTF1{i: Fin 3}
+         (op tr: (OP.oi1 i))
+         (un: HC.isUnitary tr):
       Inf (Cond.c1 op)
-          (Prog.gate1 tr)
+          (Prog.gate1 tr un)
           (Cond.c1 (LinearMap.comp (LinearMap.comp tr op) (HC.adj tr)))
-| Ax.UTF2(i1 i2: Fin 3)(ord: i1 < i2):
-    ∀op tr: (OP.oi2 i1 i2 ord),
+
+| Ax.UTF2{i1 i2: Fin 3}
+         {ord: i1 < i2}
+         (op tr: (OP.oi2 i1 i2 ord))
+         (un: HC.isUnitary tr):
       Inf (Cond.c2 op)
-          (Prog.gate2 tr)
+          (Prog.gate2 tr un)
           (Cond.c2 ((tr • op)•(HC.adj tr)))
-| Ax.Inf_1_1(i1 i2: Fin 3)(ord: i1 < i2):
-    ∀op: OP.oi1 i1, ∀s: StateReg1Ind i2,
+
+| Ax.Inf_1_1(i1 i2: Fin 3)
+            (ord: i1 < i2)
+            (op: OP.oi1 i1)
+            (s: StateReg1Ind i2):
       Inf (Cond.c1 op)
           (Prog.ass1 s)
           (Cond.c2 (TO.tpo1o1i i1 i2 ord op (OP s s)))
-| Ax.Inf_1_1_(i1 i2: Fin 3)(ord: i1 > i2):
-    ∀op: OP.oi1 i1, ∀s: StateReg1Ind i2,
+
+| Ax.Inf_1_1_(i1 i2: Fin 3)
+             (ord: i1 > i2)
+             (op: OP.oi1 i1)
+             (s: StateReg1Ind i2):
       Inf (Cond.c1 op)
           (Prog.ass1 s)
-          (Cond.c2 (TO.tpo1o1i i2 i1 ord (OP s s) op))
-| Ax.Inf_2_1(i1 i2: Fin 3)(ord: i1 < i2)(i3: Fin 3)(neq1: ¬(i1=i3))(neq2: ¬(i2=i3)):
-    ∀op: OP.oi2 i1 i2 ord, ∀s: StateReg1Ind i3,
+          (Cond.c2 (TO.tpo1o1i i2 i1 (by aesop) (OP s s) op))
+
+| Ax.Inf_2_1(i1 i2: Fin 3)
+            (ord: i1 < i2)
+            (i3: Fin 3)
+            (neq1: ¬(i1=i3))
+            (neq2: ¬(i2=i3))
+            (op: OP.oi2 i1 i2 ord)
+            (s: StateReg1Ind i3):
       Inf (Cond.c2 op)
           (Prog.ass1 s)
           (Cond.c3 (TO.tpo2o1i i1 i2 ord i3 (by aesop) (by aesop) op (OP s s)))
-| Ax.Inf_1_2(i1 i2: Fin 3)(ord: i1 < i2)(i3: Fin 3)(neq1: ¬(i1=i3))(neq2: ¬(i2=i3)):
+
+| Ax.Inf_1_2(i1 i2: Fin 3)
+            (ord: i1 < i2)
+            (i3: Fin 3)
+            (neq1: ¬(i1=i3))
+            (neq2: ¬(i2=i3)):
     ∀op: OP.oi1 i3, ∀s: StateReg2Ind i1 i2 ord,
       Inf (Cond.c1 op)
           (Prog.ass2 s)
           (Cond.c3 (TO.tpo2o1i i1 i2 ord i3 (by aesop) (by aesop) (OP s s) op))
+
 | R.SC: ∀A B C: Cond, ∀S1 S2: Prog, Inf A S1 B → Inf B S2 C → Inf A (Prog.seq S1 S2) C
+
+inductive State where
+| s1{i:Fin 3}(s: StateReg1Ind i):
+      State
+| s2{i1 i2: Fin 3}{ord: i1 < i2}(s: StateReg2Ind i1 i2 ord):
+      State
+| s3(s: StateReg3):
+      State
+
+def transforms(sBeg: State)(prog: Prog)(sFin: State): Prop :=
+match sBeg, sFin with
+| State.s1 sBeg, State.s1 sFin =>
+          (IP.f sBeg sBeg) = 1 ∧
+          (IP.f sFin sFin) = 1 ∧
+          (Inf (Cond.c1 (OP sBeg sBeg))
+               prog
+               (Cond.c1 (OP sFin sFin)))
+| State.s1 sBeg, State.s2 sFin =>
+          (IP.f sBeg sBeg) = 1 ∧
+          (IP.f sFin sFin) = 1 ∧
+          (Inf (Cond.c1 (OP sBeg sBeg))
+               prog
+               (Cond.c2 (OP sFin sFin)))
+| State.s1 sBeg, State.s3 sFin =>
+          (IP.f sBeg sBeg) = 1 ∧
+          (IP.f sFin sFin) = 1 ∧
+          (Inf (Cond.c1 (OP sBeg sBeg))
+               prog
+               (Cond.c3 (OP sFin sFin)))
+| State.s2 sBeg, State.s1 sFin =>
+          (IP.f sBeg sBeg) = 1 ∧
+          (IP.f sFin sFin) = 1 ∧
+          (Inf (Cond.c2 (OP sBeg sBeg))
+               prog
+               (Cond.c1 (OP sFin sFin)))
+| State.s2 sBeg, State.s2 sFin =>
+          (IP.f sBeg sBeg) = 1 ∧
+          (IP.f sFin sFin) = 1 ∧
+          (Inf (Cond.c2 (OP sBeg sBeg))
+               prog
+               (Cond.c2 (OP sFin sFin)))
+| State.s2 sBeg, State.s3 sFin =>
+          (IP.f sBeg sBeg) = 1 ∧
+          (IP.f sFin sFin) = 1 ∧
+          (Inf (Cond.c2 (OP sBeg sBeg))
+               prog
+               (Cond.c3 (OP sFin sFin)))
+| State.s3 sBeg, State.s1 sFin =>
+          (IP.f sBeg sBeg) = 1 ∧
+          (IP.f sFin sFin) = 1 ∧
+          (Inf (Cond.c3 (OP sBeg sBeg))
+               prog
+               (Cond.c1 (OP sFin sFin)))
+| State.s3 sBeg, State.s2 sFin =>
+          (IP.f sBeg sBeg) = 1 ∧
+          (IP.f sFin sFin) = 1 ∧
+          (Inf (Cond.c3 (OP sBeg sBeg))
+               prog
+               (Cond.c2 (OP sFin sFin)))
+| State.s3 sBeg, State.s3 sFin =>
+          (IP.f sBeg sBeg) = 1 ∧
+          (IP.f sFin sFin) = 1 ∧
+          (Inf (Cond.c3 (OP sBeg sBeg))
+               prog
+               (Cond.c3 (OP sFin sFin)))
